backend/CSEproof.v
@@ -935,6 +935,7 @@ Proof.
   (* external function *)
   simpl. econstructor; split.
   eapply exec_function_external; eauto.
+  eapply external_call_symbols_preserved; eauto. exact symbols_preserved.
   econstructor; eauto.
 
   (* return *)
